Examples/Scroll/Keccak/All.lean
@@ -5,5 +5,7 @@ import Examples.Scroll.Keccak.CellManager
 import Examples.Scroll.Keccak.Constants
 import Examples.Scroll.Keccak.Extraction
 import Examples.Scroll.Keccak.Lookups.All
+import Examples.Scroll.Keccak.MeetsConstraints
+import Examples.Scroll.Keccak.Proof
 import Examples.Scroll.Keccak.Selectors
 import Examples.Scroll.Keccak.Util
