Examples/Scroll/Keccak/Gates/Padding/StartIntermediate.lean
@@ -6,7 +6,7 @@ namespace Keccak.Gates.Padding
   lemma gate_139_padding_start_intermediate_byte (c: ValidCircuit P P_Prime) (h_fixed: c.1.Fixed = fixed_func c) (hgate: gate_139 c) (h_n: 215 < c.n):
     ∀ round ≤ 17, round > 0 →
     is_paddings c round 0 = 1 →
-    (input_bytes c round)[0]? = .some (8, is_first_padding c round 0)
+    (input_bytes c round).1[0]? = .some (8, is_first_padding c round 0)
   := by
     unfold gate_139 at hgate
     intro round hround hround_lower h_is_padding
@@ -16,7 +16,7 @@ namespace Keccak.Gates.Padding
     simp [to_cell_manager, h_n'] at hgate
     simp [is_paddings] at h_is_padding
     rewrite [h_is_padding, one_mul] at hgate
-    simp only [input_bytes, Transform.split_expr, keccak_constants, Split.expr]
+    simp only [input_bytes, Transform.split_expr, keccak_constants, Split.expr_res]
     simp [word_parts_known, List.getElem?_map, List.getElem?_enum]
     simp [is_first_padding, is_paddings, is_padding_prev, h_is_padding, cell_manager_to_raw]
     simp [cell_manager_to_raw, add_eq_zero_iff_eq_neg] at hgate
@@ -33,7 +33,7 @@ namespace Keccak.Gates.Padding
   lemma gate_141_padding_start_intermediate_byte (c: ValidCircuit P P_Prime) (h_fixed: c.1.Fixed = fixed_func c) (hgate: gate_141 c) (h_n: 215 < c.n):
     ∀ round ≤ 17, round > 0 →
     is_paddings c round 1 = 1 →
-    (input_bytes c round)[1]? = .some (8, is_first_padding c round 1)
+    (input_bytes c round).1[1]? = .some (8, is_first_padding c round 1)
   := by
     unfold gate_141 at hgate
     intro round hround hround_lower h_is_padding
@@ -43,7 +43,7 @@ namespace Keccak.Gates.Padding
     simp [to_cell_manager, h_n'] at hgate
     simp [is_paddings] at h_is_padding
     rewrite [h_is_padding, one_mul] at hgate
-    simp only [input_bytes, Transform.split_expr, keccak_constants, Split.expr]
+    simp only [input_bytes, Transform.split_expr, keccak_constants, Split.expr_res]
     simp [word_parts_known, List.getElem?_map, List.getElem?_enum]
     simp [is_first_padding, is_paddings, is_padding_prev, h_is_padding, cell_manager_to_raw]
     simp [cell_manager_to_raw, add_eq_zero_iff_eq_neg] at hgate
@@ -52,7 +52,7 @@ namespace Keccak.Gates.Padding
   lemma gate_143_padding_start_intermediate_byte (c: ValidCircuit P P_Prime) (h_fixed: c.1.Fixed = fixed_func c) (hgate: gate_143 c) (h_n: 215 < c.n):
     ∀ round ≤ 17, round > 0 →
     is_paddings c round 2 = 1 →
-    (input_bytes c round)[2]? = .some (8, is_first_padding c round 2)
+    (input_bytes c round).1[2]? = .some (8, is_first_padding c round 2)
   := by
     unfold gate_143 at hgate
     intro round hround hround_lower h_is_padding
@@ -62,7 +62,7 @@ namespace Keccak.Gates.Padding
     simp [to_cell_manager, h_n'] at hgate
     simp [is_paddings] at h_is_padding
     rewrite [h_is_padding, one_mul] at hgate
-    simp only [input_bytes, Transform.split_expr, keccak_constants, Split.expr]
+    simp only [input_bytes, Transform.split_expr, keccak_constants, Split.expr_res]
     simp [word_parts_known, List.getElem?_map, List.getElem?_enum]
     simp [is_first_padding, is_paddings, is_padding_prev, h_is_padding, cell_manager_to_raw]
     simp [cell_manager_to_raw, add_eq_zero_iff_eq_neg] at hgate
@@ -71,7 +71,7 @@ namespace Keccak.Gates.Padding
   lemma gate_145_padding_start_intermediate_byte (c: ValidCircuit P P_Prime) (h_fixed: c.1.Fixed = fixed_func c) (hgate: gate_145 c) (h_n: 215 < c.n):
     ∀ round ≤ 17, round > 0 →
     is_paddings c round 3 = 1 →
-    (input_bytes c round)[3]? = .some (8, is_first_padding c round 3)
+    (input_bytes c round).1[3]? = .some (8, is_first_padding c round 3)
   := by
     unfold gate_145 at hgate
     intro round hround hround_lower h_is_padding
@@ -81,7 +81,7 @@ namespace Keccak.Gates.Padding
     simp [to_cell_manager, h_n'] at hgate
     simp [is_paddings] at h_is_padding
     rewrite [h_is_padding, one_mul] at hgate
-    simp only [input_bytes, Transform.split_expr, keccak_constants, Split.expr]
+    simp only [input_bytes, Transform.split_expr, keccak_constants, Split.expr_res]
     simp [word_parts_known, List.getElem?_map, List.getElem?_enum]
     simp [is_first_padding, is_paddings, is_padding_prev, h_is_padding, cell_manager_to_raw]
     simp [cell_manager_to_raw, add_eq_zero_iff_eq_neg] at hgate
@@ -90,7 +90,7 @@ namespace Keccak.Gates.Padding
   lemma gate_147_padding_start_intermediate_byte (c: ValidCircuit P P_Prime) (h_fixed: c.1.Fixed = fixed_func c) (hgate: gate_147 c) (h_n: 215 < c.n):
     ∀ round ≤ 17, round > 0 →
     is_paddings c round 4 = 1 →
-    (input_bytes c round)[4]? = .some (8, is_first_padding c round 4)
+    (input_bytes c round).1[4]? = .some (8, is_first_padding c round 4)
   := by
     unfold gate_147 at hgate
     intro round hround hround_lower h_is_padding
@@ -100,7 +100,7 @@ namespace Keccak.Gates.Padding
     simp [to_cell_manager, h_n'] at hgate
     simp [is_paddings] at h_is_padding
     rewrite [h_is_padding, one_mul] at hgate
-    simp only [input_bytes, Transform.split_expr, keccak_constants, Split.expr]
+    simp only [input_bytes, Transform.split_expr, keccak_constants, Split.expr_res]
     simp [word_parts_known, List.getElem?_map, List.getElem?_enum]
     simp [is_first_padding, is_paddings, is_padding_prev, h_is_padding, cell_manager_to_raw]
     simp [cell_manager_to_raw, add_eq_zero_iff_eq_neg] at hgate
@@ -109,7 +109,7 @@ namespace Keccak.Gates.Padding
   lemma gate_149_padding_start_intermediate_byte (c: ValidCircuit P P_Prime) (h_fixed: c.1.Fixed = fixed_func c) (hgate: gate_149 c) (h_n: 215 < c.n):
     ∀ round ≤ 17, round > 0 →
     is_paddings c round 5 = 1 →
-    (input_bytes c round)[5]? = .some (8, is_first_padding c round 5)
+    (input_bytes c round).1[5]? = .some (8, is_first_padding c round 5)
   := by
     unfold gate_149 at hgate
     intro round hround hround_lower h_is_padding
@@ -119,7 +119,7 @@ namespace Keccak.Gates.Padding
     simp [to_cell_manager, h_n'] at hgate
     simp [is_paddings] at h_is_padding
     rewrite [h_is_padding, one_mul] at hgate
-    simp only [input_bytes, Transform.split_expr, keccak_constants, Split.expr]
+    simp only [input_bytes, Transform.split_expr, keccak_constants, Split.expr_res]
     simp [word_parts_known, List.getElem?_map, List.getElem?_enum]
     simp [is_first_padding, is_paddings, is_padding_prev, h_is_padding, cell_manager_to_raw]
     simp [cell_manager_to_raw, add_eq_zero_iff_eq_neg] at hgate
@@ -128,7 +128,7 @@ namespace Keccak.Gates.Padding
   lemma gate_151_padding_start_intermediate_byte (c: ValidCircuit P P_Prime) (h_fixed: c.1.Fixed = fixed_func c) (hgate: gate_151 c) (h_n: 215 < c.n):
     ∀ round ≤ 17, round > 0 →
     is_paddings c round 6 = 1 →
-    (input_bytes c round)[6]? = .some (8, is_first_padding c round 6)
+    (input_bytes c round).1[6]? = .some (8, is_first_padding c round 6)
   := by
     unfold gate_151 at hgate
     intro round hround hround_lower h_is_padding
@@ -138,7 +138,7 @@ namespace Keccak.Gates.Padding
     simp [to_cell_manager, h_n'] at hgate
     simp [is_paddings] at h_is_padding
     rewrite [h_is_padding, one_mul] at hgate
-    simp only [input_bytes, Transform.split_expr, keccak_constants, Split.expr]
+    simp only [input_bytes, Transform.split_expr, keccak_constants, Split.expr_res]
     simp [word_parts_known, List.getElem?_map, List.getElem?_enum]
     simp [is_first_padding, is_paddings, is_padding_prev, h_is_padding, cell_manager_to_raw]
     simp [cell_manager_to_raw, add_eq_zero_iff_eq_neg] at hgate
@@ -147,7 +147,7 @@ namespace Keccak.Gates.Padding
   lemma gate_153_padding_start_intermediate_byte_last_byte (c: ValidCircuit P P_Prime) (h_fixed: c.1.Fixed = fixed_func c) (hgate: gate_153 c) (h_n: 215 < c.n):
     ∀ round ≤ 16, round > 0 →
     is_paddings c round 7 = 1 →
-    (input_bytes c round)[7]? = .some (8, is_first_padding c round 7)
+    (input_bytes c round).1[7]? = .some (8, is_first_padding c round 7)
   := by
     unfold gate_153 at hgate
     intro round hround hround_lower h_is_padding
@@ -161,7 +161,7 @@ namespace Keccak.Gates.Padding
     have hround''': 12*round ≤ 311 := by linarith
     simp [Selectors.q_padding_last, hround'', hround'''] at hgate
     rewrite [h_is_padding] at hgate
-    simp only [input_bytes, Transform.split_expr, keccak_constants, Split.expr]
+    simp only [input_bytes, Transform.split_expr, keccak_constants, Split.expr_res]
     simp [word_parts_known, List.getElem?_map, List.getElem?_enum]
     simp [is_first_padding, is_paddings, is_padding_prev, h_is_padding, cell_manager_to_raw]
     simp [cell_manager_to_raw, add_eq_zero_iff_eq_neg] at hgate
