Examples/Scroll/Keccak/Spec/Asserts.lean
@@ -4,6 +4,6 @@ namespace Keccak
   section asserts
     -- NOTE: assert comment says DEFAULT_KECCAK_ROWS > (NUM_BYTES_PER_WORD + 1),
     -- but the assert states the following
-    lemma get_num_rows_per_round_assert: DEFAULT_KECCAK_ROWS > NUM_BYTES_PER_WORD := by trivial
+    lemma get_num_rows_per_round_assert: get_num_rows_per_round > NUM_BYTES_PER_WORD := by trivial
   end asserts
 end Keccak
