Examples/Scroll/Keccak/Spec/KeccakConstants.lean
@@ -1,6 +1,8 @@
 import Examples.Scroll.Keccak.Spec.Program
 
 namespace Keccak
+  @[keccak_constants] lemma get_degree_val: get_degree = 10 := rfl
+
   @[keccak_constants] lemma get_num_bits_per_absorb_lookup_val: get_num_bits_per_absorb_lookup = 6 := by
     rewrite [get_num_bits_per_absorb_lookup, get_num_bits_per_lookup]
     rewrite [Nat.log_eq_iff] <;> decide
@@ -9,10 +11,21 @@ namespace Keccak
     rewrite [get_num_bits_per_base_chi_lookup, get_num_bits_per_lookup]
     rewrite [Nat.log_eq_iff] <;> decide
 
+  @[keccak_constants] lemma get_num_bits_per_lookup_val: get_num_bits_per_base_chi_lookup = 4 := by
+    rewrite [get_num_bits_per_base_chi_lookup, get_num_bits_per_lookup]
+    rewrite [Nat.log_eq_iff] <;> decide
+
   @[keccak_constants] lemma get_num_bits_per_theta_c_lookup_val: get_num_bits_per_theta_c_lookup = 3 := by
     rewrite [get_num_bits_per_theta_c_lookup, get_num_bits_per_lookup]
     rewrite [Nat.log_eq_iff] <;> decide
 
-  @[keccak_constants] lemma rho_by_pi_num_word_parts_val : rho_by_pi_num_word_parts = 16 := by
-    simp [rho_by_pi_num_word_parts, get_num_bits_per_base_chi_lookup_val, target_part_sizes, List.length]
+  @[keccak_constants] lemma get_num_rows_per_round_val: get_num_rows_per_round = 12 := rfl
+
+  @[keccak_constants] lemma keccak_unusable_rows_val: keccak_unusable_rows = 59 := rfl
+
+  @[keccak_constants] lemma part_size_c_val: part_size_c = 3 := by simp [part_size_c, get_num_bits_per_theta_c_lookup_val]
+
+  @[keccak_constants] lemma rho_by_pi_num_word_parts_val: rho_by_pi_num_word_parts = 16 := by
+    simp [rho_by_pi_num_word_parts, rho_by_pi_target_word_sizes, rho_by_pi_part_size, get_num_bits_per_base_chi_lookup_val, target_part_sizes, NUM_BITS_PER_WORD]
+    rfl
 end Keccak
