Examples/Scroll/Keccak/Spec/Os/T1.lean
@@ -26,9 +26,9 @@ namespace Keccak
     simp only [t]
     congr
     . simp [bc, Transform.split_expr, h]
-      simp [Split.expr, part_size_c, keccak_constants, word_parts_known, List.enum]
+      simp [Split.expr_res, part_size_c, keccak_constants, word_parts_known, List.enum]
     . simp [part_size_c, keccak_constants, get_rotate_count]
-      simp [bc, keccak_constants, part_size_c, Transform.split_expr, Split.expr, word_parts_known, List.enum]
+      simp [bc, keccak_constants, part_size_c, Transform.split_expr, Split.expr_res, word_parts_known, List.enum]
       simp [List.rotateRight]
 
 end Keccak
